Add type checks

src/Core_Erlang_Auxiliaries.v
@@ -25,6 +25,7 @@ Inductive BIFCode :=
 | BLength | BTupleSize
 | BTl | BHd
 | BElement | BSetElement
+| BIsNumber | BIsInteger | BIsAtom | BIsBoolean
 | BNothing
 .
 
@@ -59,6 +60,10 @@ match s with
 | "tl"%string => BTl
 | "element"%string => BElement
 | "setelement"%string => BSetElement
+| "is_number"%string => BIsNumber
+| "is_integer"%string => BIsInteger
+| "is_atom"%string => BIsAtom
+| "is_boolean"%string => BIsBoolean
 (** anything else *)
 | _ => BNothing
 end.
@@ -318,6 +323,20 @@ match convert_string_to_code fname, params with
 | _, _ => inr (undef (VLit (Atom fname)))
 end.
 
+Definition eval_check (fname : string) (params : list Value) : ValueSequence + Exception := 
+match convert_string_to_code fname, params with
+| BIsNumber, [VLit (Integer i)]     => inl [ttrue]
+| BIsNumber, [val]                  => inl [ffalse]
+| BIsInteger, [VLit (Integer i)]    => inl [ttrue]
+| BIsInteger, [val]                 => inl [ffalse] 
+| BIsAtom, [VLit (Atom a)]          => inl [ttrue]
+| BIsAtom, [val]                    => inl [ffalse]
+| BIsBoolean, [VLit (Atom "true")]
+| BIsBoolean, [VLit (Atom "false")] => inl [ttrue]
+| BIsBoolean, [val]                 => inl [ffalse]
+| _, _              => inr (undef (VLit (Atom fname)))
+end.
+
 (* TODO: Always can be extended, this function simulates inter-module calls *)
 Definition eval (fname : string) (params : list Value) (eff : SideEffectList) 
    : ((ValueSequence + Exception) * SideEffectList) :=
@@ -333,6 +352,7 @@ match convert_string_to_code fname with
 | BTupleSize                                      => (eval_tuple_size params, eff)
 | BHd | BTl                                       => (eval_hd_tl fname params, eff)
 | BElement | BSetElement                          => (eval_elem_tuple fname params, eff)
+| BIsNumber | BIsInteger | BIsAtom | BIsBoolean   => (eval_check fname params, eff)
 (** anything else *)
 | BNothing                                        => (inr (undef (VLit (Atom fname))), eff)
 end.
@@ -347,7 +367,7 @@ Proof.
   destruct (convert_string_to_code fname) eqn:Hfname; simpl in H.
   all: try (unfold eval_arith, eval_logical, eval_equality,
              eval_transform_list, eval_list_tuple, eval_cmp,
-             eval_hd_tl, eval_elem_tuple in H; rewrite Hfname in H; destruct vals;
+             eval_hd_tl, eval_elem_tuple, eval_check in H; rewrite Hfname in H; destruct vals;
     [ inversion H; exists []; rewrite app_nil_r; auto |
       destruct v; try (destruct vals; inversion H; exists []; rewrite app_nil_r; auto) ]).
   * unfold eval_io in H; rewrite Hfname in H; destruct (length vals) eqn:Hl; inversion H.
@@ -375,10 +395,10 @@ Proof.
   unfold eval. destruct (convert_string_to_code fname) eqn:Hfname.
   all: try ( unfold eval_arith, eval_logical, eval_equality,
              eval_transform_list, eval_list_tuple, eval_cmp,
-             eval_hd_tl, eval_elem_tuple; rewrite Hfname; destruct vals; 
+             eval_hd_tl, eval_elem_tuple, eval_check; rewrite Hfname; destruct vals; 
              [ exists eff | simpl; auto ]).
   all: simpl; auto.
-  1-6,9-30: exists eff; auto.
+  1-6,9-34: exists eff; auto.
   * unfold eval_io. rewrite Hfname. destruct (length vals).
     - exists eff. auto.
     - destruct n. eexists. simpl. reflexivity.
@@ -398,7 +418,7 @@ Proof.
   unfold eval in *. destruct (convert_string_to_code fname) eqn:Hfname.
   all: try (unfold eval_arith, eval_logical, eval_equality,
              eval_transform_list, eval_list_tuple, eval_cmp,
-             eval_hd_tl, eval_elem_tuple in *; rewrite Hfname in *; destruct vals;
+             eval_hd_tl, eval_elem_tuple, eval_check in *; rewrite Hfname in *; destruct vals;
     simpl in *; rewrite <- app_nil_r in H at 1; apply app_inv_head in H; subst;
              rewrite app_nil_r; reflexivity).
   * unfold eval_io in *. rewrite Hfname in *. destruct (length vals).
@@ -434,7 +454,7 @@ Proof.
   unfold eval. destruct (convert_string_to_code fname) eqn:Hfname.
   all: try (unfold eval_arith, eval_logical, eval_equality,
              eval_transform_list, eval_list_tuple, eval_cmp,
-             eval_hd_tl, eval_elem_tuple; rewrite Hfname; destruct vals;
+             eval_hd_tl, eval_elem_tuple, eval_check; rewrite Hfname; destruct vals;
     [ reflexivity |
       destruct v; try (destruct vals; auto) ]).
   * unfold eval_io. rewrite Hfname. destruct (length vals).
@@ -473,7 +493,7 @@ Proof.
   unfold eval. destruct (convert_string_to_code f) eqn:Hfname.
   all: try (unfold eval_arith, eval_logical, eval_equality,
              eval_transform_list, eval_list_tuple, eval_cmp,
-             eval_hd_tl, eval_elem_tuple; rewrite Hfname; destruct vals; auto).
+             eval_hd_tl, eval_elem_tuple, eval_check; rewrite Hfname; destruct vals; auto).
   * unfold eval_io. rewrite Hfname. destruct (length vals).
     - simpl. auto.
     - destruct n.
@@ -841,6 +861,33 @@ Proof. reflexivity. Qed.
 Goal (eval "setelement" [ttrue; ttrue; ttrue]) [] = (inr (badarg (VTuple [VLit (Atom "setelement"); ttrue; ttrue; ttrue])), []).
 Proof. unfold eval, eval_elem_tuple. simpl. reflexivity. Qed.
 Goal (eval "setelement" [ttrue]) [] = (inr (undef (VLit (Atom "setelement"))), []).
+Proof. reflexivity. Qed.
+
+Goal eval "is_number" [VLit (Integer 2)] [] = (inl [ttrue], []).
+Proof. reflexivity. Qed.
+Goal eval "is_number" [ffalse] [] = (inl [ffalse], []).
+Proof. reflexivity. Qed.
+Goal eval "is_number" [ffalse; ffalse] [] = (inr (undef (VLit (Atom "is_number"))), []).
+Proof. reflexivity. Qed.
+Goal eval "is_integer" [VLit (Integer 2)] [] = (inl [ttrue], []).
+Proof. reflexivity. Qed.
+Goal eval "is_integer" [ffalse] [] = (inl [ffalse], []).
+Proof. reflexivity. Qed.
+Goal eval "is_integer" [ffalse; ffalse] [] = (inr (undef (VLit (Atom "is_integer"))), []).
+Proof. reflexivity. Qed.
+Goal eval "is_atom" [VLit (Integer 2)] [] = (inl [ffalse], []).
+Proof. reflexivity. Qed.
+Goal eval "is_atom" [VLit (Atom "foo")] [] = (inl [ttrue], []).
+Proof. reflexivity. Qed.
+Goal eval "is_atom" [ffalse; ffalse] [] = (inr (undef (VLit (Atom "is_atom"))), []).
+Proof. reflexivity. Qed.
+Goal eval "is_boolean" [VLit (Integer 2)] [] = (inl [ffalse], []).
+Proof. reflexivity. Qed.
+Goal eval "is_boolean" [ttrue] [] = (inl [ttrue], []).
+Proof. reflexivity. Qed.
+Goal eval "is_boolean" [ffalse] [] = (inl [ttrue], []).
+Proof. reflexivity. Qed.
+Goal eval "is_boolean" [ffalse; ffalse] [] = (inr (undef (VLit (Atom "is_boolean"))), []).
 Proof. reflexivity. Qed.
 
 End Tests.
